progress

core_deduction.v
@@ -25,6 +25,12 @@ where "A ⊢c p" := (cnd A p).
 Lemma dne A p : A ⊢c (¬¬p) -> A ⊢c p.
 Proof. intro. now apply cndDN, ndDN. Defined.
 
+Lemma dni A p : A ⊢ p -> A ⊢ (¬¬p).
+Proof. intro. apply ndI, ndII, ndI, (ndIE _ _ _ _ p).
+  -apply ndI,ndHyp. now left.
+  -now apply (weakening A), incl_tl.
+Defined.
+
 Fixpoint weakening_c A B p (H : A ⊢c p) : incl A B -> B ⊢c p.
 Proof. destruct  H; intro Hinc;
   [ now apply cndI, (weakening_imp form _ cnd weakening_c A)
@@ -51,25 +57,57 @@ Proof. destruct p.
   -apply translation_subst_univ. { intro. reflexivity. } { intros. reflexivity. } apply translation_subst.
 Defined.
 
+Lemma cut A p q : A ⊢ p -> (p :: A) ⊢ q -> A ⊢ q.
+Proof.
+  intros. apply ndI,(ndIE _ _ _ _ p). now apply ndI,ndII. now apply (weakening A).
+Qed.
+
+Lemma cut_c A p q : A ⊢c p -> (p :: A) ⊢c q -> A ⊢c q.
+Proof.
+  intros. apply cndI,(ndIE _ _ _ _ p). now apply cndI,ndII. now apply (weakening_c A).
+Qed.
+
+Lemma subst_helper p: subst_form (var_term 0, var_term) (subst_form (up_term_term (S >> var_term)) p) = p.
+Proof. fsimpl. Admitted.
+(*  destruct p; destruct f; cbn; unfold up_term_term. *)
+
+Fixpoint translation_helper A p : A ⊢ (¬¬«p») -> A ⊢ «p».
+Proof. destruct p; cbn; intros.
+  -apply (translation_helper_imp _ _ _ weakening _ ndI). {intros. now apply translation_helper. } assumption.
+  -eapply (translation_helper_univ _ _ subst_form). {intros. reflexivity. } apply ndU. apply cut. apply subst_helper.
+   {intros. reflexivity. } apply ndI. intros. now apply translation_helper. assumption.
+Defined.
+
+Lemma translation_dn p : «¬¬p» = ¬¬«p».
+Proof. now reflexivity. Defined.
+
 Fixpoint translation_fwd A p (H : A ⊢c p) : «/A» ⊢ «p».
 Proof. destruct H; [apply ndI | apply ndU | ].
   -apply (translation_imp _  nd cnd). {intro. reflexivity. } apply translation_fwd. assumption.
   -apply (translation_univ _ nd cnd). {intro. reflexivity. } apply translation_subst. apply translation_fwd. assumption.
-  -apply (translation_class _ nd cnd retract_form_implicative_form). apply dne. apply translation_fwd. assumption.
-(* Defined.
- *)Admitted.
+  -destruct H. apply translation_helper. rewrite <- translation_dn. now apply translation_fwd.
+Defined.
 
-Fixpoint translation_bwd A (p : form) : «/A» ⊢c «p» -> A ⊢c p.
-Proof. destruct p; cbn; intro.
-  -apply (translation_bwd_imp _ retract_form_implicative_form _ translate). {intro. reflexivity. } apply translation_bwd. assumption.
-  -apply (translation_bwd_univ _ retract_form_universal_form _ translate). {intro. reflexivity. } apply translation_bwd. assumption.
-(* Defined.
- *)Admitted.
+Fixpoint translation_bwd A (p : form) : A ⊢c «p» <-> A ⊢c p.
+Proof. destruct p; cbn.
+  -apply (translation_bwd_imp  _ retract_form_implicative_form _ translate).
+   apply cndI. apply cut_c. apply translation_bwd.
+  -eapply (translation_bwd_univ _ retract_form_universal_form subst_form ). {intros. reflexivity. }
+   apply cndU. apply cut_c. apply subst_helper. apply cndI. apply translation_bwd.
+Defined.
+
+Lemma translation_rm_ctx A B p : (A ++ «/B») ⊢c p -> (A ++ B) ⊢c p.
+Proof. revert A. induction B; cbn; [auto |].
+  intros. specialize (IHB (A ++ (cons a nil))). do 2 rewrite <- app_assoc in IHB. apply IHB. apply cut_c with («a»).
+    -apply translation_bwd. apply cndI,ndHyp,in_or_app. right. now left.
+    -apply (weakening_c _ _ _ H). unfold incl. intros. destruct (in_app_or _ _ _ H0). right. apply in_or_app. now left.
+     destruct H1. now left. right. apply in_or_app. right. apply in_or_app. now right.
+Defined.
 
 Theorem translation A p: A ⊢c p <-> «/A» ⊢ «p».
 Proof. split.
   -apply translation_fwd.
-  -intro. now apply translation_bwd, embed.
+  -intro. apply translation_rm_ctx with (A := nil). now apply translation_bwd, embed.
 Qed.
 
 End translation.
