existential_deduction.v
@@ -17,16 +17,18 @@ Section Existential.
   Variable nd : list form -> form -> Prop.
   Notation "A ⊢ p" := (nd A p) (at level 70).
 
+  Definition up_ctx (A : list form) := map (subst_form (S >> var_term)) A.
   Inductive nd_exst (A : list form) : form -> Prop :=
     | ndEI p t : A ⊢ subst_form (scons t (var_term)) p -> A ⊢_exst (∃ p)
-    | ndEE p q : A ⊢ (∃ p) -> p :: A ⊢ q -> A ⊢_exst q
+    | ndEE p q : A ⊢ (∃ p) -> p :: (up_ctx A) ⊢ subst_form (S >> var_term) q -> A ⊢_exst q
   where "A ⊢_exst p" := (nd_exst A p).
 
   Variable weakening : forall A B p, A ⊢ p -> incl A B -> B ⊢ p.
   Lemma weakening_exst A B p : A ⊢_exst p -> incl A B -> B ⊢_exst p.
-  Proof. destruct 1; intro Hinc; [ now apply (ndEI _ p t), (weakening A) | apply (ndEE _ p q) ].
+  Proof. revert B. destruct 1; intro Hinc; [ now apply (ndEI _ p t), (weakening A) | apply (ndEE _ p q) ].
     -now apply (weakening A).
-    -apply (weakening (p::A)), incl_cons; [assumption | now left | now apply incl_tl ].
+    -apply (weakening (p::up_ctx A)), incl_cons; [assumption | now left | apply incl_tl ].
+      unfold up_ctx. now apply incl_map.
   Defined.
 
   Variable retract_implicative : included form_implicative form.
@@ -38,20 +40,26 @@ Section Existential.
   Notation "« p »" := (translate p).
   Notation "«/ A »" := (map translate A).
 
+
   Variable agree : forall A p, A ⊢_exst p -> A ⊢ p.
-  Variable dne : forall A p, A ⊢ (¬¬p) -> A ⊢ p.
-  Variable dni : forall A p, A ⊢ p -> A ⊢ (¬¬p).
-  Variable subst_var: forall p, subst_form (var_term 0, var_term) p = p.
+  Variable agree_cls : forall A p, nd_classic _ _ nd A p -> A ⊢ p.
+  Variable agree_imp : forall A p, nd_imp _ _ nd A p -> A ⊢ p.
   Variable imp_nd : forall A p, nd_imp _ _ nd A p -> A ⊢ p.
+  Variable subst_form_inj : forall sigma p, subst_form sigma (inj p) = subst_form_existential _ subst_form _ sigma p.
   Variable translation_inj : forall p, «inj p» = translate_exst  p.
-  Variable translation_bwd : forall A p, «/A» ⊢ «p» -> A ⊢ p.
-  Lemma translation_bwd_exst A p: «/A» ⊢ (translate_exst p) -> A ⊢ inj p.
-  Proof. destruct p; cbn. intro. apply dne in H. apply (ndEE _ _ «∃ f») in H. now apply translation_bwd, agree.
-    -rewrite translation_inj. cbn. now apply dni, (weakening «/A»), incl_tl.
+  Variable aux : forall p, subst_form (scons (var_term 0) (var_term)) (subst_form (up_term_term (S >> var_term)) p) = p.
+  Variable translation_bwd : forall A p, A ⊢ «p» <-> A ⊢ p.
+  Lemma translation_bwd_exst A p: A ⊢ (translate_exst p) <-> A ⊢ inj p.
+  Proof. destruct p. cbn. split; intro.
+    - assert (Hc : A ⊢ ∃ «f»). {now apply agree_cls,ndDN. }
+      apply (ndEE _ _ (∃ f)) in Hc. now apply agree. rewrite subst_form_inj. cbn. apply agree,(ndEI _ _ (var_term 0)).
+      rewrite aux. apply translation_bwd, agree_imp,ndHyp. now left.
+    -apply agree_imp,ndII,agree_imp,(ndIE _ _ _ _ (∃«f»)). apply agree_imp,ndHyp. now left.
+      apply (weakening A). 2:now apply incl_tl. apply (ndEE _ _ (∃«f»)) in H. now apply agree.
+      rewrite subst_form_inj. cbn. apply agree,(ndEI _ _ (var_term 0)). rewrite aux. apply translation_bwd.
+      apply agree_imp,ndHyp. now left.
   Defined.
 
-
-  Variable subst_form_inj : forall sigma p, subst_form sigma (inj p) = subst_form_existential _ subst_form _ sigma p.
   Variable subst_dn : forall sigma p, subst_form sigma (¬¬p) = ¬¬(subst_form sigma p).
   Variable translation_subst : forall sigma q, «subst_form sigma q» = subst_form sigma «q».
   Lemma translation_subst_exst sigma p :  « subst_form_existential _ subst_form _ sigma p » = subst_form sigma (translate_exst p).
@@ -59,6 +67,16 @@ Section Existential.
     rewrite subst_form_inj. cbn. apply congr_Exist_; apply translation_subst. all: reflexivity.
   Defined.
 
+  Variable cut : forall A p q,  A ⊢ p -> (p :: A) ⊢ q -> A ⊢ q.
+  Lemma translation_helper_exst A p : A ⊢ (¬¬(translate_exst p)) -> A ⊢ translate_exst p.
+  Proof. destruct p. cbn. intro. apply (cut _ _ _ H). apply agree_imp,ndII,agree_imp,(ndIE _ _ _ _ (¬¬¬(∃«f»))).
+    apply agree_imp,ndHyp. right. now left. apply agree_imp,ndII,agree_imp,(ndIE _ _ _ _ (¬(∃«f»))).
+    apply agree_imp,ndHyp. now left. apply agree_imp,ndHyp. right. now left.
+  Defined.
+
+  Lemma translation_map A: up_ctx «/A» = «/up_ctx A».
+  Proof. unfold up_ctx. repeat rewrite map_map. apply map_ext. intro p. symmetry. apply translation_subst.
+  Qed.
 End Existential.
 
 Section translation.
@@ -84,18 +102,29 @@ Section translation.
   Proof. destruct 1. now apply (ndEI _ _ _ _ _ _ t), embed. apply (ndEE _ _ _ _ _ p); now apply embed.
   Defined.
 
-  Variable imp_nd : forall A p, nd_imp form _ (nd_exst _ _ subst_form nd) A p -> A ⊢[nd] p.
   Variable weakening : forall A B p, nd A p -> incl A B -> nd B p.
 
-  Lemma dn_int_exst A p: A ⊢[nd] p -> A ⊢[nd] (¬¬p).
+(*   Lemma dn_int_exst A p: A ⊢[nd] p -> A ⊢[nd] (¬¬p).
   Proof. intro. apply imp_nd, ndII, imp_nd, (ndIE _ _ _ _ p).
     -apply imp_nd, ndHyp. now left.
     -now apply (weakening_exst _ _ _ _ weakening A), incl_tl.
-  Qed.
+  Qed. *)
+  Variable dni : forall A p, nd A p -> nd A (¬¬p).
+
+  Variable agree_cnd : forall A p, A ⊢[cnd] p -> cnd A p.
+  Variable agree_nd : forall A p, A ⊢[nd] p -> nd A p. 
+  Variable agree_cls : forall A p, nd_classic _ _ cnd A p -> cnd A p.
+  Variable agree_imp : forall A p, nd_imp _ _ nd A p -> nd A p.
+ Variable aux : forall p, subst_form (scons (var_term 0) (var_term)) (subst_form (up_term_term (S >> var_term)) p) = p.
+
   Variable translation : forall A p, cnd A p -> nd «/A» «p».
   Lemma translation_exst A p: A ⊢[cnd] p -> «/A» ⊢[nd] «p».
   Proof. destruct 1.
-    -rewrite translation_inj. apply dn_int_exst, (ndEI _ _ _ _ _ _ t). rewrite <- translation_subst. now apply translation.
-    -apply (ndEE _ _ _ _ _ «p»). admit. rewrite <- map_cons. now apply translation.
+    -rewrite translation_inj. cbn. admit.
+    -apply (ndEE _ _ _ _ _ «(subst_form (up_term_term (S >> var_term)) p)»).  apply agree_nd, (ndEI _ _ _ _ _ _ (var_term 0)).
+      rewrite <- translation_subst. rewrite aux. apply translation. admit.
+      rewrite <- translation_subst. rewrite translation_map. rewrite <- map_cons. apply translation.
+      apply agree_cnd,(ndEE _ _ _ _ _ p).
+
   Admitted.
 End translation.
