universal_deduction.v
@@ -1,7 +1,7 @@
 Require Export unscoped header_extensible.
 
 Require Export implicativesyntax universalsyntax termsyntax.
-Require Import classical_deduction.
+Require Import classical_deduction implicative_deduction.
 
 Reserved Notation "A ⊢ p" (at level 70).
 Reserved Notation "A ⊢_univ p" (at level 70).
@@ -47,9 +47,31 @@ Section universals.
   Proof. destruct p. cbn. rewrite subst_form_inj. unfold All_. rewrite translation_inj. cbn. apply congr_All_, translation_subst.
   Defined.
 
-  Variable translation_bwd : forall A p,  «/A» ⊢ «p» -> A ⊢ p.
-  Lemma translation_bwd_univ A p: «/A» ⊢ translate_univ p -> A ⊢ inj p.
-  Proof. destruct p; cbn; intro; apply translation_bwd; rewrite translation_inj; auto.
+  Variable agree : forall A p, nd_univ A p -> A ⊢ p.
+  Variable  cut : forall A p q, A ⊢ p -> (p :: A) ⊢ q -> A ⊢ q.
+  Variable aux : forall p, subst_form (scons (var_term 0) (var_term)) (subst_form (up_term_term (S >> var_term)) p) = p.
+
+  Variable retract_imp : retract (form_implicative form) form.
+  Variable subst_form_inj_imp : forall sigma p, subst_form sigma (inj p) = subst_form_implicative _ subst_form _ sigma p.
+  Variable agree_imp : forall A p, nd_imp _ _ nd A p -> A ⊢ p.
+  Variable translation_bwd : forall A p,  A ⊢ «p» <-> A ⊢ p.
+  Lemma translation_bwd_univ A p: A ⊢ translate_univ p <-> A ⊢ inj p.
+  Proof. destruct p. cbn. split; intro; apply (cut _ _ _ H), agree,ndUI,translation_bwd; cbn;
+    rewrite subst_form_inj; cbn; rewrite <- aux;
+    apply agree,ndUE, agree_imp,ndHyp; now left.
+  Defined.
+
+  Lemma translation_map A: up_ctx «/A» = «/up_ctx A».
+  Proof. unfold up_ctx. repeat rewrite map_map. apply map_ext. intro p. symmetry. apply translation_subst.
+  Qed.
+  Variable translation_helper : forall p A, A ⊢ (¬¬«p») -> A ⊢ «p».
+  Lemma translation_helper_univ A p : A ⊢ (¬¬(translate_univ p)) -> A ⊢ translate_univ p.
+  Proof. intro H. apply (cut _ _ _ H). destruct p. cbn. apply agree,ndUI, translation_helper. cbn.
+    repeat (rewrite subst_form_inj_imp; cbn ).
+    apply agree_imp,ndII,agree_imp,(ndIE _ _ _ _ (¬(subst_form (S >> var_term) (∀«f»)))).
+    apply agree_imp,ndHyp. right. now left.
+    apply agree_imp,ndII,agree_imp,(ndIE _ _ _ _ «f»). apply agree_imp,ndHyp. right. now left.
+    rewrite subst_form_inj. cbn. rewrite <- aux. apply agree,ndUE,agree_imp,ndHyp. now left.
   Defined.
 
 End universals.
@@ -77,14 +99,11 @@ Section translation.
   Proof. destruct q. rewrite translation_subst. rewrite translation_inj. auto.
   Defined. *)
 
-  Lemma translation_map A: up_ctx form subst_form (map translate A) = map translate (up_ctx form subst_form A).
-  Proof. unfold up_ctx. repeat rewrite map_map. apply map_ext. intro p. symmetry. apply translation_subst.
-  Qed.
 
   Variable translation : forall A p, cnd A p -> nd «/A» «p».
   Lemma translation_univ A p: A ⊢[cnd] p -> «/A» ⊢[nd] «p».
   Proof. destruct 1.
-    -rewrite translation_inj. cbn. apply ndUI. rewrite translation_map. now apply translation.
+    -rewrite translation_inj. cbn. apply ndUI. rewrite translation_map. now apply translation. now apply translation_subst.
     -rewrite translation_subst. apply ndUE. { pose (translation_inj (All _ p)). cbn in e. rewrite <- e. now apply translation. }
   Defined.
 
